src/Pipit.System.Ind.fst
@@ -13,104 +13,122 @@ let rec prop_for_all (l: list prop): prop =
 let all_checks_hold (#input #state #value: Type) (t: system input state value) (s: state): prop =
   prop_for_all (List.Tot.map (fun (n, i) -> i s) t.chck)
 
+let system_holds (#input #state #value: Type) (t: system input state value): prop =
+  forall (inputs: list (input & value)) (s: state).
+    Cons? inputs            ==>
+    system_stepn t inputs s ==>
+    all_checks_hold t s
+
 let base_case (#input #state #value: Type) (t: system input state value): prop =
   forall (i: input) (s: state) (s': state) (r: value).
     t.init s ==> t.step i s s' r ==>
     all_checks_hold t s'
+
+let rec base_case_k' (k: nat) (#input #state #value: Type) (t: system input state value) (s': state) (check: prop): prop =
+  match k with
+  | 0 -> t.init s' ==> check
+  | _ ->
+    forall (i: input) (s: state) (r: value).
+      t.step i s s' r ==>
+      base_case_k' (k - 1) t s check
+
+let rec base_case_k (k: nat) (#input #state #value: Type) (t: system input state value): prop =
+  (if k > 1 then base_case_k (k - 1) t else True) /\
+  (forall (s': state). base_case_k' k t s' (all_checks_hold t s'))
 
 let step_case (#input #state #value: Type) (t: system input state value): prop =
   forall (i0 i1: input) (s0: state) (s1 s2: state) (r0 r1: value).
     t.step i0 s0 s1 r0 ==> all_checks_hold t s1 ==>
     t.step i1 s1 s2 r1 ==> all_checks_hold t s2
 
-// WRONG quantifiers in the wrong place
-let rec step_case_k' (k: nat) (#input #state #value: Type) (t: system input state value) (s': state): prop =
+let rec step_case_k' (k: nat) (#input #state #value: Type) (t: system input state value) (s': state) (check: prop): prop =
   match k with
-  | 0 ->
-    forall (i: input) (s: state) (r: value).
-        t.step i s s' r ==>
-        all_checks_hold t s'
-  | _ ->
-  forall (i: input) (s: state) (r: value).
-    step_case_k' (k - 1) t s ==>
+  | 0 -> check
+  | _ -> forall (i: input) (s: state) (r: value).
     t.step i s s' r ==>
-    all_checks_hold t s'
-
-// let rec step_case_k' (k: nat) (#input #state #value: Type) (t: system input state value) (s': state): prop =
-//   forall (i: input) (s: state) (r: value).
-//     let step' =
-//       if k = 0
-//       then True
-//       else step_case_k' (k - 1) t s
-//     in
-//     step' ==>
-//     t.step i s s' r ==>
-//     all_checks_hold t s'
+    all_checks_hold t s ==>
+    step_case_k' (k - 1) t s check
 
 let step_case_k (k: nat) (#input #state #value: Type) (t: system input state value): prop =
-  forall (s': state). step_case_k' k t s'
-
-// let chk (t: system 'i 's 'v): unit =
-//   assert (step_case t == step_case_k 1 t) by (FStar.Tactics.norm [nbe; delta; zeta; iota; primops]; FStar.Tactics.norm [delta_fully ["Pipit.System.Ind.step_case_k"; "Pipit.System.Ind.step_case_k'"]]; FStar.Tactics.dump "ok")
-
-let step_case_2 (#input #state #value: Type) (t: system input state value): prop =
-  forall (i0 i1 i2: input) (s0 s1 s2 s3: state) (r0 r1 r2: value).
-    t.step i0 s0 s1 r0 ==> all_checks_hold t s1 ==>
-    t.step i1 s1 s2 r1 ==> all_checks_hold t s2 ==>
-    t.step i2 s2 s3 r2 ==> all_checks_hold t s3
-
-let step_case_3 (#input #state #value: Type) (t: system input state value): prop =
-  forall (i0 i1 i2 i3: input) (s0 s1 s2 s3 s4: state) (r0 r1 r2 r3: value).
-    t.step i0 s0 s1 r0 ==> all_checks_hold t s1 ==>
-    t.step i1 s1 s2 r1 ==> all_checks_hold t s2 ==>
-    t.step i2 s2 s3 r2 ==> all_checks_hold t s3 ==>
-    t.step i3 s3 s4 r3 ==> all_checks_hold t s4
-
-let step_case_4 (#input #state #value: Type) (t: system input state value): prop =
-  forall (i0 i1 i2 i3 i4: input) (s0: state) (s1 s2 s3 s4 s5: state) (r0 r1 r2 r3 r4: value).
-    t.step i0 s0 s1 r0 ==> all_checks_hold t s1 ==>
-    t.step i1 s1 s2 r1 ==> all_checks_hold t s2 ==>
-    t.step i2 s2 s3 r2 ==> all_checks_hold t s3 ==>
-    t.step i3 s3 s4 r3 ==> all_checks_hold t s4 ==>
-    t.step i4 s4 s5 r4 ==> all_checks_hold t s5
+  forall (s': state). step_case_k' k t s' (all_checks_hold t s')
 
 let induct1 (#input #state #value: Type)
   (t: system input state value): prop =
     base_case t /\ step_case t
 
-// let rec induct1_sound (#len: nat) (#input #state: Type)
-//   (t: system input state prop)
-//   (inputs: C.vector input len)
-//   (props: C.vector prop len)
-//   (s': state):
-//     Lemma
-//         (requires system_stepn t inputs props s' /\ induct1 t)
-//         (ensures prop_for_all props) =
-//  match inputs, props with
-//  | [], [] -> ()
-//  | [i], [p] -> ()
-//  | i1 :: i0 :: is, p1 :: p0 :: ps ->
-//    assert (len >= 2);
-//    eliminate exists (s0: state) (s1: state).
-//      system_stepn #(len - 2) t is ps s0 /\
-//      t.step i0 s0 s1 p0
-//    returns prop_for_all props
-//    with h.
-//      induct1_sound #(len - 1) t (i0 :: is) (p0 :: ps) s1
+let rec induct1_sound' (#input #state #value: Type)
+  (t: system input state value)
+  (inputs: list (input & value))
+  (s': state):
+    Lemma
+        (requires system_stepn t inputs s' /\ induct1 t /\ Cons? inputs)
+        (ensures all_checks_hold t s')
+        (decreases inputs) =
+  match inputs with
+  | [] -> ()
+  | [(i, v)] -> ()
+  | (i1,v1) :: (i0,v0) :: ivs ->
+    eliminate exists (s0: state) (s1: state).
+      system_stepn t ivs s0 /\
+      t.step i0 s0 s1 v0 /\
+      t.step i1 s1 s' v1
+    returns all_checks_hold t s'
+    with h.
+      (induct1_sound' t ((i0, v0) :: ivs) s1)
 
-// let bmc2' (#input #state: Type) (t: system input state C.value): prop =
-//   forall (i1 i2: input) (s0 s1 s2: state) (r1 r2: C.value).
-//     t.init s0 ==>
-//     t.step i1 s0 s1 r1 ==>
-//     t.step i2 s1 s2 r2 ==>
-//     r2 <> 0
+let induct1_sound (#input #state #value: Type)
+  (t: system input state value):
+    Lemma
+        (requires induct1 t)
+        (ensures system_holds t) =
+  introduce forall (inputs: list (input & value) { Cons? inputs }) (s: state { system_stepn t inputs s }).
+    (Cons? inputs) ==>
+    system_stepn t inputs s ==>
+    all_checks_hold t s
+  with
+    (induct1_sound' t inputs s)
 
-// let bmc2 (#input #state: Type) (t: system input state prop): prop =
-//   forall (i1 i2: input) (s0 s1 s2: state) (r1 r2: prop).
-//     t.init s0 ==>
-//     t.step i1 s0 s1 r1 ==>
-//     t.step i2 s1 s2 r2 ==>
-//     r2
+let induct_k (k: nat) (#input #state #value: Type)
+  (t: system input state value): prop =
+    base_case_k k t /\ step_case_k k t
+
+let rec induct2_sound' (#input #state #value: Type)
+  (t: system input state value)
+  (inputs: list (input & value))
+  (s': state):
+    Lemma
+        (requires system_stepn t inputs s' /\ induct_k 2 t)
+        (ensures Nil? inputs \/ all_checks_hold t s')
+        (decreases inputs) =
+  match inputs with
+  | [] -> ()
+  | [(i0, v0)] -> ()
+  | [(i0, v0); (i1, v1)] -> ()
+  | (i2,v2) :: (i1,v1) :: (i0,v0) :: ivs ->
+    eliminate exists (s0: state) (s1: state) (s2: state).
+      system_stepn t ivs s0 /\
+      t.step i0 s0 s1 v0 /\
+      t.step i1 s1 s2 v1 /\
+      t.step i2 s2 s' v2
+    returns all_checks_hold t s'
+    with h.
+      (induct2_sound' t ((i1, v1) :: (i0, v0) :: ivs) s2;
+      induct2_sound' t ((i0, v0) :: ivs) s1;
+      ())
+
+let induct2_sound (#input #state #value: Type)
+  (t: system input state value):
+    Lemma
+        (requires induct_k 2 t)
+        (ensures system_holds t) =
+  introduce forall (inputs: list (input & value) { Cons? inputs }) (s: state { system_stepn t inputs s }).
+    (Cons? inputs) ==>
+    system_stepn t inputs s ==>
+    all_checks_hold t s
+  with
+    (induct2_sound' t inputs s)
+
+// TODO inductk_sound
 
 (* Shelved: proof that properties proved for transition systems apply to original expression *)
 // open Pipit.Exp.Base
@@ -133,7 +151,6 @@ let induct1 (#input #state #value: Type)
 // let rec prop_for_all__prop_of_bool (vs: list value):
 //   Lemma (requires prop_for_all (C.vector_map #(List.Tot.length vs) prop_of_value vs))
 //         (ensures List.Tot.for_all (fun r -> r <> 0) vs) =
-//  admit ()
 
 // let induct1_exp (#vars: nat)
 //   (e: exp { exp_valid e vars }):
